ExistentialRules/ChaseSequence/ChaseTree.lean
@@ -24,55 +24,60 @@ public section
 variable {sig : Signature} [DecidableEq sig.P] [DecidableEq sig.C] [DecidableEq sig.V]
 
 /-- The `ChaseTree` merely extends the `TreeDerivation` with the condition that the root is the database from the knowledge base. -/
-structure ChaseTree (obs : ObsolescenceCondition sig) (kb : KnowledgeBase sig) extends TreeDerivation obs kb.rules where
-  database_first : tree.root = some {
-    facts := kb.db.toFactSet
-    origin := none
-    facts_contain_origin_result := by simp
-  }
+structure ChaseTree (N : Type u) (obs : ObsolescenceCondition sig) (kb : KnowledgeBase sig) [CN : ChaseNode N obs kb.rules] extends TreeDerivation N obs kb.rules where
+  -- We do not need to demand existence here since the TreeDerivation already ensures that the root exists.
+  -- The ∀ quantifier makes this condition more convenient to use.
+  database_first : ∀ root ∈ tree.root,
+    CN.ingoingFacts root = kb.db.toFactSet ∧
+    CN.outgoingFacts root = kb.db.toFactSet ∧
+    CN.origin root = none
 
 namespace ChaseTree
 
 variable {obs : ObsolescenceCondition sig} {kb : KnowledgeBase sig}
 
-instance : Membership (ChaseNode obs kb.rules) (ChaseTree obs kb) where
+instance {N : Type u} [CN : ChaseNode N obs kb.rules] : Membership N (ChaseTree N obs kb) where
   mem td node := node ∈ td.tree
 
 /-- An element is a member of the tree iff it occurs at some address. -/
-theorem mem_iff {ct : ChaseTree obs rules} : ∀ {e}, e ∈ ct ↔ ∃ ns, ct.tree.get? ns = some e := TreeDerivation.mem_iff
+theorem mem_iff {N : Type u} [CN : ChaseNode N obs kb.rules] {ct : ChaseTree N obs kb} :
+  ∀ {e}, e ∈ ct ↔ ∃ ns, ct.tree.get? ns = some e := TreeDerivation.mem_iff
 
 /-- We can convert `ChaseDerivation`s that are branches in the `ChaseTree` to `ChaseBranch`es. -/
 @[expose]
-def chaseBranch_for_branch {ct : ChaseTree obs kb} {branch : ChaseDerivation obs kb.rules} (branch_mem : branch ∈ ct.branches) : ChaseBranch obs kb := {
+def chaseBranch_for_branch {N : Type u} [CN : ChaseNode N obs kb.rules] {ct : ChaseTree N obs kb} {branch : ChaseDerivation N obs kb.rules} (branch_mem : branch ∈ ct.branches) : ChaseBranch N obs kb := {
   branch := branch.branch
   isSome_head := branch.isSome_head
   triggers_exist := branch.triggers_exist
   triggers_active := branch.triggers_active
   fairness := branch.fairness
   database_first := by
-    rw [← ct.database_first]
     rw [TreeDerivation.branches_eq] at branch_mem
-    have head := branch_mem.left
-    unfold TreeDerivation.root ChaseDerivationSkeleton.head at head; rw [Option.get_inj] at head; exact head
+    have head_eq := branch_mem.left
+    unfold TreeDerivation.root ChaseDerivationSkeleton.head at head_eq; rw [Option.get_inj] at head_eq
+    intro head; rw [head_eq]
+    exact ct.database_first head
 }
 
 /-- We restate the `database_first` condition in terms of the `TreeDerivation` vocabulary. -/
-theorem database_first' {ct : ChaseTree obs kb} : ct.root = {
-  facts := kb.db.toFactSet,
-  origin := none,
-  facts_contain_origin_result := by simp
-} := by simp only [TreeDerivation.root, ct.database_first, Option.get_some]
+theorem database_first' {N : Type u} [CN : ChaseNode N obs kb.rules] {ct : ChaseTree N obs kb} :
+    CN.ingoingFacts ct.root = kb.db.toFactSet ∧
+    CN.outgoingFacts ct.root = kb.db.toFactSet ∧
+    CN.origin ct.root = none := by
+  apply ct.database_first; simp [TreeDerivation.root]
 
 /-- Opposed to a `TreeDerivation`, we know that each node in a `ChaseBranch` has a finite set of facts. This is because the database is finite and each trigger only adds finitely many new facts. -/
-theorem facts_finite_of_mem {ct : ChaseTree obs kb} {node : ChaseNode obs kb.rules} (node_mem : node ∈ ct) : node.facts.finite := by
+theorem facts_finite_of_mem {ct : ChaseTree (RegularChaseNode obs kb.rules) obs kb} {node : RegularChaseNode obs kb.rules} (node_mem : node ∈ ct) :
+    node.facts.finite := by
   rw [ct.facts_node_eq_union_initial_and_generated node_mem]
   apply Set.union_finite_of_both_finite
-  . rw [database_first']; exact kb.db.toFactSet.property.left
+  . rw [← ct.root.outgoingFacts_eq, database_first'.right.left]; exact kb.db.toFactSet.property.left
   . exact ct.generatedFacts_finite_of_mem node_mem
 
 /-- The root of the `ChaseTree` does not contain any function terms. -/
-theorem func_term_not_mem_root {ct : ChaseTree obs kb} {t : GroundTerm sig} (t_is_func : ∃ func ts arity_ok, t = GroundTerm.func func ts arity_ok) :
-    ¬ t ∈ ct.root.facts.terms := by
+theorem func_term_not_mem_root {N : Type u} [CN : ChaseNode N obs kb.rules] {ct : ChaseTree N obs kb}
+    {t : GroundTerm sig} (t_is_func : ∃ func ts arity_ok, t = GroundTerm.func func ts arity_ok) :
+    ¬ t ∈ (CN.outgoingFacts ct.root).terms := by
   intro t_mem
   simp only [database_first'] at t_mem
   rcases t_mem with ⟨f, f_mem, t_mem⟩
@@ -82,7 +87,7 @@ theorem func_term_not_mem_root {ct : ChaseTree obs kb} {t : GroundTerm sig} (t_i
   simp [GroundTerm.func_neq_const] at t_eq
 
 /-- Each element of the result of a `ChaseTree` not only models the rule set but the whole `KnowledgeBase`. -/
-theorem result_models_kb {ct : ChaseTree obs kb} : ∀ fs ∈ ct.result, fs.modelsKb kb := by
+theorem result_models_kb {ct : ChaseTree (RegularChaseNode obs kb.rules) obs kb} : ∀ fs ∈ ct.result, fs.modelsKb kb := by
   unfold TreeDerivation.result; simp only [Set.mem_map]
   intro fs ⟨branch, branch_mem, fs_mem⟩
   let cb := ct.chaseBranch_for_branch branch_mem
@@ -91,15 +96,16 @@ theorem result_models_kb {ct : ChaseTree obs kb} : ∀ fs ∈ ct.result, fs.mode
   exact cb.result_models_kb
 
 /-- Constants in the chase must be in the database or in some rule. -/
-theorem constants_node_subset_constants_db_union_constants_rules {ct : ChaseTree obs kb} {node : ChaseNode obs kb.rules} (node_mem : node ∈ ct) :
+theorem constants_node_subset_constants_db_union_constants_rules {ct : ChaseTree (RegularChaseNode obs kb.rules) obs kb}
+    {node : RegularChaseNode obs kb.rules} (node_mem : node ∈ ct) :
     node.facts.constants ⊆ (kb.db.constants.val ∪ kb.rules.head_constants) := by
   have := ct.constants_node_subset_constants_fs_union_constants_rules node_mem
-  simp only [ct.database_first', Database.toFactSet_constants_same] at this
+  rw [← ct.root.outgoingFacts_eq, ct.database_first'.right.left, Database.toFactSet_constants_same] at this
   exact this
 
 /-- Each functional term in the chase originates as a fresh term from a trigger. -/
 theorem functional_term_originates_from_some_trigger
-    {ct : ChaseTree obs kb}
+    {ct : ChaseTree (RegularChaseNode obs kb.rules) obs kb}
     (node : ct.NodeWithAddress)
     {t : GroundTerm sig}
     (t_is_func : ∃ func ts arity_ok, t = GroundTerm.func func ts arity_ok)
@@ -111,7 +117,7 @@ theorem functional_term_originates_from_some_trigger
 
 /-- If a functional term occurs in the chase, then the trigger that introduces this term must have been used in the chase. -/
 theorem trigger_introducing_functional_term_occurs_in_chase
-    {ct : ChaseTree obs kb}
+    {ct : ChaseTree (RegularChaseNode obs kb.rules) obs kb}
     (node : ct.NodeWithAddress)
     {t : GroundTerm sig}
     (t_mem_node : t ∈ node.node.facts.terms)
@@ -126,7 +132,7 @@ theorem trigger_introducing_functional_term_occurs_in_chase
 
 /-- If a functional term occurs in the chase, then the result of the trigger that introduces this term is contained in the current node. -/
 theorem result_of_trigger_introducing_functional_term_occurs_in_chase
-    {ct : ChaseTree obs kb}
+    {ct : ChaseTree (RegularChaseNode obs kb.rules) obs kb}
     (node : ct.NodeWithAddress)
     {t : GroundTerm sig}
     (t_mem_node : t ∈ node.node.facts.terms)
